You are an expert math teacher and IMO coach.

There are basically two methods of writing math problems:

- **Backwards**: It involves taking some basic idea, technique, or method X, and constructing a problem specifically using X. Examples include problems like "Not like a G6" (reverse-engineered from a complex number identity) and "2012-2013 Fall OMO #28" (using silly algebraic manipulations). This method can relatively quickly generate many "acceptable" questions, but the resulting problems often feel artificial.
- **Forwards**: It is less about intentionally trying to write problems and more about genuinely exploring math. It involves actions such as generalizing existing results, finding analogs of familiar ideas in new contexts, refining hypotheses, or focusing on a particular aspect of a proof. Examples include "2012-2013 Fall OMO #29", "2012-2013 Fall OMO #25", "2013-2014 USA December TST #2", and "2013 ELMO #3". This method is considered the most natural way to generate interesting and motivated problems.

Given a problem and a reference answer, please

1. Clearly restate variables, hypotheses, and the final conclusion (final answer) of the problem in Lean 4;
2. Try to solve the problem in natural language;
3. Identify which pattern the problem is constructed in, express the problem design process as a Markov decision process in Lean 4, and summarize the action sequence.

- **State**: the "problem design" state maintains variables, hypotheses, and conclusions.
- **Action**: two actions: _introduce_ and _deduce_. - _Introduce_: add new variables or hypotheses into the state (`have`statement by `sorry`); - _Deduce_: deduce new conclusions from the state (`have`statement by a concrete proof).

The following is an example

# Problem

In $\triangle ABC$, the sides opposite to angles $A$, $B$, $C$ are denoted as $a$, $b$, $c$ respectively, and $\overrightarrow{m}=(\sqrt{3}b-c,\cos C)$, $\overrightarrow{n}=(a,\cos A)$. Given that $\overrightarrow{m} \parallel \overrightarrow{n}$, determine the value of $\cos A$.

# Answer

\dfrac{\sqrt{3}}{3}

# Analysis

## Problem Statement

```
import Mathlib

example
  -- $ABC$ is a triangle
  (A B C : ℝ)
  (h_triangle_sum : A + B + C = Real.pi)
  (h_triangle_A : 0 < A ∧ A < Real.pi)
  (h_triangle_B : 0 < B ∧ B < Real.pi)
  (h_triangle_C : 0 < C ∧ C < Real.pi)
  -- the sides opposite to angles $A$, $B$, $C$ are denoted as $a$, $b$, $c$
  (a b c : ℝ)
  (h_pos_a : a > 0)
  (h_pos_b : b > 0)1111
  (h_pos_c : c > 0)
  (h_triangle_ab : a / Real.sin A = b / Real.sin B)
  (h_triangle_bc : b / Real.sin B = c / Real.sin C)
  -- $\\\\overrightarrow{m}=(\\\\sqrt{3}b-c,\\\\cos C)$, $\\\\overrightarrow{n}=(a,\\\\cos A)$
  (m n : ℝ × ℝ)
  (hm : m = (Real.sqrt 3 * b - c, Real.cos C))
  (hn : n = (a, Real.cos A))
  -- $\\\\overrightarrow{m} \\\\parallel \\\\overrightarrow{n}$
  (h_parallel : m.1 * n.2 = m.2 * n.1)
  -- determine the value of $\\\\cos A$.
  (answer : ℝ)
  (h_answer : answer = Real.cos A)
  -- # Answer \\\\dfrac{\\\\sqrt{3}}{3}
: (answer = Real.sqrt 3 / 3)
:= by sorry
1111
```

## Action Sequence

```
  -- introduce a triangle and let $A$, $B$, $C$ represent the angles of it
  have A : ℝ := by sorry
  have B : ℝ := by sorry
  have C : ℝ := by sorry
  have h_triangle_sum : A + B + C = Real.pi := by sorry
  have h_triangle_A : 0 < A ∧ A < Real.pi := by sorry
  have h_triangle_B : 0 < B ∧ B < Real.pi := by sorry
  have h_triangle_C : 0 < C ∧ C < Real.pi := by sorry
  -- introduce the sides opposite to angles $A$, $B$, $C$, denoted as $a$, $b$, $c$
  have a : ℝ := by sorry
  have b : ℝ := by sorry
  have c : ℝ := by sorry
  have h_pos_a : a > 0 := by sorry
  have h_pos_b : b > 0 := by sorry
  have h_pos_c : c > 0 := by sorry
  have h_triangle_ab : a / Real.sin A = b / Real.sin B := by sorry
  have h_triangle_bc : b / Real.sin B = c / Real.sin C := by sorry
  -- introduce two vectors $\\overrightarrow{m}=(\\sqrt{3}b-c,\\cos C)$, $\\overrightarrow{n}=(a,\\cos A)$
  have m : ℝ × ℝ := by sorry
  have n : ℝ × ℝ := by sorry
  have hm : m = (Real.sqrt 3 * b - c, Real.cos C) := by sorry
  have hn : n = (a, Real.cos A) := by sorry
  -- introduce the condition that $\\overrightarrow{m} \\parallel \\overrightarrow{n}$
  have h_parallel : m.1 * n.2 = m.2 * n.1 := by sorry
  -- deduce the condition h_triangle by substituting the values of m and n into h_parallel
  have h_triangle : (Real.sqrt 3 * b - c)*(Real.cos A) = (Real.cos C)*a := by
    rw [hm, hn] at h_parallel
    exact h_parallel
  -- deduce the condition h_cos_A and h_cos_C according to the Cosine Law
  have h_cos_A : Real.cos A = (b^2+c^2-a^2)/(2*b*c) := by sorry
  have h_cos_C : Real.cos C = (a^2+b^2-c^2)/(2*a*b) := by sorry
  -- deduce the condition h_triangle_simp by substituting h_cos_A and h_cos_B into h_triangle and simplifying
  have h_triangle_simp : (Real.sqrt 3 * b - c)*(b^2+c^2-a^2)=(a^2+b^2-c^2)*c := by
    rw [h_cos_A, h_cos_C] at h_triangle
    have heq1 : (√3 * b - c) * ((b ^ 2 + c ^ 2 - a ^ 2) / (2 * b * c)) = (a ^ 2 + b ^ 2 - c ^ 2) / (2 * a * b) * a := by
      linarith [h_triangle]
    have heq2 : (a ^ 2 + b ^ 2 - c ^ 2) / (2 * a * b) * a = (a ^ 2 + b ^ 2 - c ^ 2) / (2 * b) := by
      field_simp [show a ≠ 0 by linarith, show b ≠ 0 by linarith]
      all_goals nlinarith
    rw [heq2] at heq1
    have h1 : b ≠ 0 := by linarith
    have h2 : c ≠ 0 := by linarith
    have heq3 : (√3 * b - c) * ((b ^ 2 + c ^ 2 - a ^ 2) / (2 * b * c)) * (2 * b) = (a ^ 2 + b ^ 2 - c ^ 2) / (2 * b) * (2 * b) := by
      rw [heq1]
    have heq4 : (√3 * b - c) * ((b ^ 2 + c ^ 2 - a ^ 2) / (2 * b * c)) * (2 * b) = (√3 * b - c) * ((b ^ 2 + c ^ 2 - a ^ 2) / c) := by
      field_simp [show b ≠ 0 by linarith, show c ≠ 0 by linarith]
      all_goals nlinarith
    have heq5 : (a ^ 2 + b ^ 2 - c ^ 2) / (2 * b) * (2 * b) = a ^ 2 + b ^ 2 - c ^ 2 := by
      field_simp [show b ≠ 0 by linarith]
    rw [heq4, heq5] at heq3
    have heq6 : (√3 * b - c) * (b ^ 2 + c ^ 2 - a ^ 2) = (a ^ 2 + b ^ 2 - c ^ 2) * c := by
      have h3 : c ≠ 0 := by linarith
      field_simp [h3] at heq3
      rw [heq3]
    exact heq6
  -- deduce the condition h_a_square by further simplifying the expression h_triangle_simp and expressing a^2
  have h_a_square : a^2 = b^2 + c^2 - 2/Real.sqrt 3 * b * c := by
    have h1 : 0 < √3 := by positivity
    have h2 : √3 > 0 := by positivity
    have eq1 : (√3 * b - c) * (b ^ 2 + c ^ 2 - a ^ 2) = (a ^ 2 + b ^ 2 - c ^ 2) * c := by linarith [h_triangle_simp]
    have eq2 : √3 * b ^ 3 + √3 * b * c ^ 2 - √3 * a ^ 2 * b - c * b ^ 2 - c ^ 3 + a ^ 2 * c = a ^ 2 * c + b ^ 2 * c - c ^ 3 := by
      nlinarith [eq1, sq_pos_of_pos h_pos_b, sq_pos_of_pos h_pos_c, sq_pos_of_pos h_pos_a, Real.sqrt_pos.mpr (show (3 : ℝ) > 0 by norm_num), Real.sq_sqrt (show (0 : ℝ) ≤ (3 : ℝ) by norm_num)]
    have eq3 : √3 * b ^ 3 + √3 * b * c ^ 2 - √3 * a ^ 2 * b - c * b ^ 2 - b ^ 2 * c = 0 := by
      nlinarith [eq2, sq_pos_of_pos h_pos_b, sq_pos_of_pos h_pos_c, sq_pos_of_pos h_pos_a, Real.sqrt_pos.mpr (show (3 : ℝ) > 0 by norm_num), Real.sq_sqrt (show (0 : ℝ) ≤ (3 : ℝ) by norm_num)]
    have eq4 : b * (√3 * b ^ 2 + √3 * c ^ 2 - √3 * a ^ 2 - c * b - b * c) = 0 := by
      nlinarith [eq3, sq_pos_of_pos h_pos_b, sq_pos_of_pos h_pos_c, sq_pos_of_pos h_pos_a, Real.sqrt_pos.mpr (show (3 : ℝ) > 0 by norm_num), Real.sq_sqrt (show (0 : ℝ) ≤ (3 : ℝ) by norm_num)]
    cases' (mul_eq_zero.mp eq4) with hb h5
    · -- Case where b = 0, which contradicts h_pos_b
      exfalso
      linarith
    · -- Case where the second factor is zero
      have eq6 : √3 * b ^ 2 + √3 * c ^ 2 - √3 * a ^ 2 - c * b - b * c = 0 := by
        nlinarith
      have eq7 : √3 * (b ^ 2 + c ^ 2 - a ^ 2) = 2 * b * c := by
        nlinarith [eq6, sq_pos_of_pos h_pos_b, sq_pos_of_pos h_pos_c, sq_pos_of_pos h_pos_a, Real.sqrt_pos.mpr (show (3 : ℝ) > 0 by norm_num), Real.sq_sqrt (show (0 : ℝ) ≤ (3 : ℝ) by norm_num)]
      have eq8 : b ^ 2 + c ^ 2 - a ^ 2 = (2 * b * c) / √3 := by
        have h9 : √3 ≠ 0 := by positivity
        field_simp
        nlinarith [eq7, Real.sqrt_pos.mpr (show (3 : ℝ) > 0 by norm_num), Real.sq_sqrt (show (0 : ℝ) ≤ (3 : ℝ) by norm_num)]
      have eq9 : a ^ 2 = b ^ 2 + c ^ 2 - 2 / √3 * b * c := by
        have h10 : √3 > 0 := by positivity
        have eq10 : (2 * b * c) / √3 = (2 / √3) * b * c := by
          field_simp
          all_goals ring
        nlinarith [eq8, eq10, Real.sqrt_pos.mpr (show (3 : ℝ) > 0 by norm_num), Real.sq_sqrt (show (0 : ℝ) ≤ (3 : ℝ) by norm_num)]
      exact_mod_cast eq9
  -- deduce the answer that Real.cos A = Real.sqrt 3 / 3 by substituting h_a_square into h_cos_A
  have h_answer : Real.cos A = Real.sqrt 3 / 3 := by
    rw [h_cos_A, h_a_square]
    field_simp [show b ≠ 0 by linarith, show c ≠ 0 by linarith]
    have h1 : √3 ^ 2 = 3 := by
      rw [Real.sq_sqrt]
      norm_num
    calc
      2 * b * c * 3 = 6 * b * c := by ring
      _ = √3 * (√3 * (2 * b * c)) := by
        have h2 : √3 * (√3 * (2 * b * c)) = (√3 ^ 2) * (2 * b * c) := by
          ring
        rw [h2]
        rw [h1]
        ring
```

**Note :**

```
  -- deduce the condition h_cos_A and h_cos_C according to the Cosine Law
  have h_cos_A : Real.cos A = (b^2+c^2-a^2)/(2*b*c) := by sorry
  have h_cos_C : Real.cos C = (a^2+b^2-c^2)/(2*a*b) := by sorry
```

这里其实是Deduce，但由于Lean当中有关三角形的定理比较少，难以证明

# Problem

Let $m$ and $n$ be 2 integers such that $m>n$. Suppose $m+n=20$, $m^2+n^2=328$, find $m^2-n^2$.

# Answer

320

## Problem Statement

```
import Mathlib

example
  -- $m$ and $n$ are 2 integers 
  (m n : Int)
  -- $m > n$
  (hmn : m > n)
  -- $m+n=20$ and $m^2+n^2=328$
  (h_sum : m+n=20)
  (h_square_sum : m^2+n^2=328)
  -- find the value of $m^2-n^2$
  (answer : Int)
  (h_answer : answer=m^2-n^2)
  -- # Answer 320
 : (answer = 320)
 := by sorry
```

## Action Sequence

```
  -- introduce two integers m and n 
  have m : Int := by sorry
  have n : Int := by sorry
  -- introduce the condition that m > n 
  have hmn : m > n := by sorry
  -- introduce the condition that m+n=20 
  have h_sum : m + n = 20 := by sorry
  -- introduce the condition that m^2+n^2=328
  have h_square_sum : m^2 + n^2 = 328 := by sorry
  -- deduce the condition m*n=36 from h_sum and h_square_sum
  have h_mul : m * n = 36 := by
    have : (m + n)^2 = m^2 + n^2 + 2 * m * n := by ring
    rw [h_sum, h_square_sum] at this
    linarith
  -- deduce the condition (m-n)^2 = 256 from h_square_sum and h_mul
  have h_diff_square : (m - n)^2 = 256 := by
    have : (m - n)^2 = m^2 + n^2 - 2 * (m * n) := by ring
    rw [h_square_sum, h_mul] at this
    linarith
  -- deduce the condition m-n=16 from h_diff_square and hmn 
  have h_diff : m - n = 16 := by
    nlinarith
  -- deduce the answer that m^2-n^2 = 320 from h_sum and h_diff
  have h_answer : m^2 - n^2 = 320 := by
    nlinarith1
```

# Problem

Find all primes that can be written both as a sum of two primes and as a difference of two primes.

# Answer

5

## Problem Statement

```
import Mathlib

example 
	-- $p,q,r,s,t$ are five primes
	(p q r s t : Nat)
	(hp : p.Prime)
	(hq : q.Prime)
	(hr : r.Prime)
	(hs : s.Prime)
	(ht : t.Prime)
	-- $p$ can be expressed as the difference of $q$ and $r$
	(heq1 : p = q - r)
	-- $p$ can be expressed as the sum of $s$ and $t$
	(heq2 : p = s + t)
	-- find the value of $p$
	(answer : Nat)
	(h_answer : answer = p)
	-- # Answer 5
: answer = 5
:= by sorry
```

## Action Sequence

```
  -- introduce five primes $p, q, r, s, t$
  have p : Nat := by sorry
  have q : Nat := by sorry
  have r : Nat := by sorry
  have s : Nat := by sorry
  have t : Nat := by sorry
  have hp : p.Prime := by sorry
  have hq : q.Prime := by sorry
  have hr : r.Prime := by sorry
  have hs : s.Prime := by sorry
  have ht : t.Prime := by sorry
  -- induction the condition that t > s
  have hle1 : t > s := by sorry
  -- induction the condition that p = q - r
  have heq1 : p = q - r := by sorry
  -- deduce the condition that q > r
  have hle2 : q > r := by
    by_contra h
    have : p = 0 := by
      rw [heq1]
      omega
    apply Nat.Prime.ne_zero hp this
  -- induction the condition that p = s + t
  have heq2 : p = s + t := by sorry
  -- deduce the condition that p > 2
  have hge : p > 2 := by
    rw [heq2]
    have : s ≥ 2 := by exact Nat.Prime.two_le hs
    have : t ≥ 2 := by exact Nat.Prime.two_le ht
    linarith
  -- deduce the condition that p is odd
  have hoddp : Odd p := by
    by_contra h
    simp at h
    have : p = 2 := by exact (Nat.Prime.even_iff hp).mp h
    linarith
  -- deduce the condition that r = 2
  have heqr : r = 2 := by
    have : Even q ∨ Even r := by
      rw [heq1] at hoddp
      by_contra h
      simp at h
      have : Even (q-r) := Nat.Odd.sub_odd h.1 h.2
      have : ¬ Odd (q-r) := by exact Nat.not_odd_iff_even.mpr this
      contradiction
    rcases this with h1 | h2
    · have : q = 2 := by exact (Nat.Prime.even_iff hq).mp h1
      rw [this] at hle2
      have : r ≥ 2 := by exact Nat.Prime.two_le hr
      linarith
    · exact (Nat.Prime.even_iff hr).mp h2
  -- deduce the condition that either s or t is even
  have heven : Even s ∨ Even t := by
    rw [heq2] at hoddp
    by_contra h
    simp at h
    have : Even (s + t) := Odd.add_odd h.1 h.2
    have : ¬ Odd (s+t) := by exact Nat.not_odd_iff_even.mpr this
    contradiction
  -- deduce the condition that s is Even.
  have hevens : Even s := by
    rcases heven with h1 | h2
    · exact h1
    · have : t = 2 := by exact (Nat.Prime.even_iff ht).mp h2
      have : s ≥ 2 := by exact Nat.Prime.two_le hs
      linarith
  -- duduce the condition that s = 2
  have heqs : s = 2 := by exact (Nat.Prime.even_iff hs).mp hevens
  -- duduce the condition that t is 3 by considering the possible values of t modulo 3
  have heqt : t = 3 := by
    have : t % 3 = 0 ∨ t % 3 = 1 ∨ t % 3 = 2 := by
      by_contra h
      simp at h
      have : t % 3 ≥ 3 := by
        rcases h with ⟨h1, h2, h3⟩
        apply Nat.add_one_le_iff.mpr
        apply Nat.two_lt_of_ne
        · apply h1
        · apply h2
        · apply h3
      have : t % 3 < 3 := Nat.mod_lt t (by norm_num)
      linarith
    rcases this with h1 | h2 | h3
    · have : 3 ∣ t := by exact Nat.dvd_of_mod_eq_zero h1
      symm
      apply (Nat.dvd_prime_two_le ht (by linarith)).mp this
    · have : p % 3 = 0 := by
        rw [heq2, heqs, Nat.add_mod 2 t 3, h2]
      have : 3 ∣ p := by exact Nat.dvd_of_mod_eq_zero this
      have : p = 3 := by
        symm
        apply (Nat.dvd_prime_two_le hp (by linarith)).mp this
      have : t = 1 := by
        calc
          _ = p - s := by rw [heq2]; norm_num
          _ = 3 - 2 := by rw [this, heqs]
      rw [this] at heq2
      have := Nat.Prime.ne_one ht this
      exact False.elim this
    · have : q % 3 = 0 := by
        calc
          _ = (p + r) % 3 := by
            rw [heq1]
            rw [Nat.sub_add_cancel (by linarith)]
          _ = (s + t + r) % 3 := by rw [heq2]
          _ = _ := by
            rw [Nat.add_mod]
            rw [Nat.add_mod s t 3]
            rw [heqs, h3, heqr]
      have : 3 ∣ q := by exact Nat.dvd_of_mod_eq_zero this
      have : q = 3 := by
        symm
        apply (Nat.dvd_prime_two_le hq (by linarith)).mp this
      rw [this, heqr] at heq1
      simp at heq1
      rw [heq1] at hge
      linarith
  -- deduce the answer that p = 5
	  have h_answer : p = 5 := by
    omega
```

# Problem

There exist real numbers $x$ and $y$ , both greater than 1, such that $\log_x (y^x) = \log_y (x^{(4y)}) = 10$. Find $xy$

# Answer

25

## Problem Statement

```
import Mathlib

example
	-- $x, y$ are two real numbers
	(x y : Real)
	-- $x, y$ are both greater than 1
	(hx : x > 1)
	(hy : y > 1)
	-- $\\log_x (y^x) = \\log_y (x^(4y)) = 10$
	(hxy1 : Real.logb x (y^x) = 10)
	(hxy2 : Real.logb y (x^(4*y)) = 10)
	-- find the value of $xy$
	(answer : Real)
	(h_answer : answer = x*y)
	-- # Answer 25
: answer = 25
:= by sorry
```

## Action Sequence

```
  -- introduce two real numbers x and y
  have x : Real := by sorry
  have y : Real := by sorry
  -- introduce the condition that x and y are both greater than 1
  have hx : x > 1 := by sorry
  have hy : y > 1 := by sorry
  -- introduce the condition that $\\log_x (y^x) = \\log_y (x^(4y)) = 10$
  have hxy1 : Real.logb x (y^x) = 10 := by sorry
  have hxy2 : Real.logb y (x^(4*y)) = 10 := by sorry
  -- deduce that x * Real.logb x y = 10
  have hxy3 : x * Real.logb x y = 10 := by
    rw [← hxy1]
    rw [Real.logb_rpow_eq_mul_logb_of_pos]
    linarith
  -- deduce that 4 * y * Real.logb y x = 10
  have hxy4 : 4 * y * Real.logb y x = 10 := by
    rw [← hxy2]
    rw [Real.logb_rpow_eq_mul_logb_of_pos]
    linarith
  -- deduce that 4 * x * y * Real.logb x y * Real.logb y x = 100 by multiplying the two equations
  have hxy5 : 4 * x * y * (Real.logb x y * Real.logb y x) = 100 := by
    nlinarith
  -- deduce that 4 * x * y = 100 according to the equation that Real.logb x y * Real.logb y x = 1
  have hxy6 : 4 * x * y = 100 := by
    rw [Real.mul_logb (by linarith) (by linarith) (by linarith)] at hxy5
    rw [Real.logb_self_eq_one (by linarith)] at hxy5
    nlinarith
  -- deduce the answer that x * y = 25
  have h_answer : x * y = 25 := by
    nlinarith

```

# Problem

Suppose that the set {1,2, ..., 1998} has been partitioned into disjoint pairs {a_i, b_i} (1 ≤ i ≤ 999) so that for all i, |a_i - b_i| equals 1 or 6. Find that the sum |a_1 - b_1| + |a_2 - b_2| + ... + |a_999 - b_999| ends in which digit.

# Answer

9

## Problem Statement

```
import Mathlib 

example 
	-- s is the index set {1,2,..., 999}
	(s : Finset ℤ) 
	(hs : s = Finset.Icc 1 999)
	-- a and b are two sequence 
	(a b : Int -> Int)
	-- the set {1,2, ..., 1998} has been partitioned into disjoint pairs {a_i, b_i} (1 ≤ i ≤ 999)
	(ha : ∀ i ∈ s, a i ∈ Finset.Icc 1 1998)
	(hb : ∀ i ∈ s, b i ∈ Finset.Icc 1 1998)
	(hij : ∀ i ∈ s, ∀ j ∈ s, i ≠ j → a i ≠ a j ∧ b i ≠ b j)
	(hij' : ∀ i ∈ s, ∀ j ∈ s, a i ≠ b j)
	-- |a_i - b_i| equals 1 or 6
	(habs : ∀ i ∈ s, |a i - b i| = 1 ∨ |a i - b i| = 6)
	-- Find that the sum |a_1 - b_1| + |a_2 - b_2| + ... + |a_999 - b_999| ends in which digit
	(answer : Int)
	(h_answer : answer = (∑ i ∈ s, |a i - b i|) % 10)
	-- # Answer 9
	: answer = 9 
:= by sorry

```

## Action Sequence

```
  -- introduce two sequences a and b
  have a : Int -> Int := by sorry
  have b : Int -> Int := by sorry
  -- introduce the index set s = {1, 2, ..., 999}
  have s : Finset Int := by sorry
  have hs : s = Finset.Icc 1 999 := by sorry
  -- introduce the properties of a and b : the set {1,2, ..., 1998} has been partitioned into disjoint pairs {a_i, b_i} (1 ≤ i ≤ 999)
  have ha : ∀ i ∈ s, a i ∈ Finset.Icc 1 1998 := by sorry
  have hb : ∀ i ∈ s, b i ∈ Finset.Icc 1 1998 := by sorry
  have hij : ∀ i ∈ s, ∀ j ∈ s, i ≠ j → a i ≠ a j ∧ b i ≠ b j := by sorry
  have hij' : ∀ i ∈ s, ∀ j ∈ s, a i ≠ b j := by sorry
  -- introduce the property of the differences
  have habs : ∀ i ∈ s, |a i - b i| = 1 ∨ |a i - b i| = 6 := by sorry
  -- deduce that the equation |a i - b i| % 2 = (a i + b i) % 2
  have heq : ∀ i ∈ s, |a i - b i| % 2 = (a i + b i) % 2 := by
    intro x hx
    by_cases hge : a x ≥ b x
    · have : |a x - b x| = a x - b x := by
        rw [@abs_eq_self]
        linarith
      rw [this]
      apply Int.modEq_iff_dvd.mpr
      ring_nf
      exact Int.dvd_mul_left (b x) 2
    · have : |a x - b x| = - (a x - b x) := by
        rw [@abs_eq_neg_self]
        linarith
      rw [this]
      apply Int.modEq_iff_dvd.mpr
      ring_nf
      exact Int.dvd_mul_left (a x) 2
  -- deduce that the sum of differences mod 2 is equal to the sum of (a_i + b_i) mod 2
  have heqsum : (∑ i ∈ s, |a i - b i|) % 2 = (∑ i ∈ s, (a i + b i)) % 2 := by
    rw [Finset.sum_int_mod]
    nth_rw 2 [Finset.sum_int_mod]
    rw [Finset.sum_congr rfl heq]
  -- deduce that the sum of differences is odd according to the former equation
  have hmod2 : (∑ i ∈ s, |a i - b i|) % 2 = 1 := by
    have hainj : ∀ x ∈ s, ∀ y ∈ s, a x = a y → x = y := by
      intro x hx y hy hxy
      norm_cast at hx hy
      by_contra hneq
      exact (hij x hx y hy hneq).1 hxy
    have hbinj : ∀ x ∈ s, ∀ y ∈ s, b x = b y → x = y := by
      intro x hx y hy hxy
      norm_cast at hx hy
      by_contra hneq
      exact (hij x hx y hy hneq).2 hxy
    have hdisjoint : Disjoint (Finset.image a s) (Finset.image b s) := by
      unfold Disjoint
      intro x hxa hxb
      intro y hy
      have hya : y ∈ Finset.image a s := by exact hxa hy
      have hyb : y ∈ Finset.image b s := by exact hxb hy
      simp at hya hyb
      rcases hya with ⟨z1, hz1in, hz1eq⟩
      rcases hyb with ⟨z2, hz2in, hz2eq⟩
      have := hij' z1 hz1in z2 hz2in
      rw [hz1eq, hz2eq] at this
      norm_num at this
    have hunion : Finset.image a s ∪ Finset.image b s = Finset.Icc 1 1998 := by
      have hacard : Finset.card (Finset.image a s) = 999 := by
        rw [Finset.card_image_of_injOn hainj]
        rw [hs]
        simp
      have hbcard : Finset.card (Finset.image b s) = 999 := by
        rw [Finset.card_image_of_injOn hbinj]
        rw [hs]
        simp
      have hcard : Finset.card (Finset.image a s ∪ Finset.image b s) = 1998 := by
        rw [Finset.card_union_eq_card_add_card.mpr hdisjoint, hacard, hbcard]
      symm
      refine (Finset.eq_iff_card_ge_of_superset ?hst).mp ?_
      · intro x hx
        simp at hx
        rcases hx with hx1 | hx2
        · rcases hx1 with ⟨y, hyin, hyeq⟩
          have := ha y hyin
          rw [hyeq] at this
          exact this
        · rcases hx2 with ⟨y, hyin, hyeq⟩
          have := hb y hyin
          rw [hyeq] at this
          exact this
      simp
      rw [hcard]
    let f : ℤ → ℤ := fun x => x
    have haeq : ∑ i ∈ s, a i = ∑ j ∈ Finset.image a s, j := by
      have := @Finset.sum_image ℤ ℤ ℤ f _ _ s a hainj
      unfold f at this
      rw [this]
    have hbeq : ∑ i ∈ s, b i = ∑ j ∈ Finset.image b s, j := by
      have := @Finset.sum_image ℤ ℤ ℤ f _ _ s b hbinj
      unfold f at this
      rw [this]
    have heq : ∑ i ∈ s, (a i + b i) = (∑ j ∈ Finset.image a s, j) + (∑ j ∈ Finset.image b s, j) := by
      rw [Finset.sum_add_distrib, haeq, hbeq]
    have := @Finset.sum_disjUnion ℤ ℤ (Finset.image a s) (Finset.image b s) f _ hdisjoint
    simp at this
    rw [← this, hunion] at heq
    unfold f at heq
    rw [heqsum, heq]
    rfl
  -- deduce that the sum of differences mod 5 is 4
  have hmod5 : (∑ i ∈ s, |a i - b i|) % 5 = 4 := by
    rw [Finset.sum_int_mod]
    have : ∀ i ∈ s, |a i - b i| % 5 = 1 := by
      intro i hi
      have := habs i hi
      rcases this with h1 | h2
      · rw [h1]
        norm_num
      · rw [h2]
        norm_num
    rw [Finset.sum_congr rfl this]
    rw [hs]
    simp
  -- deduce the answer is 9
  have hsum : (∑ i ∈ s, |a i - b i|) % 10 = 9 := by
    have : 10 ∣ ((∑ i ∈ s, |a i - b i|) - 9) := by
      have h2dvd : 2 ∣ ((∑ i ∈ s, |a i - b i|) - 9) := by
        exact Int.ModEq.dvd (id (Eq.symm hmod2))
      have h5dvd : 5 ∣ ((∑ i ∈ s, |a i - b i|) - 9) := by
        exact Int.ModEq.dvd (id (Eq.symm hmod5))
      apply IsCoprime.mul_dvd (by norm_num) h2dvd h5dvd
    exact id (Int.ModEq.symm (Int.modEq_of_dvd this))
```